---
layout: post
title:  "Completing the Square - Quadratic Formula, Equation, Method, Examples"
author: sal
categories: [ maths ]
image: assets/images/completing-square.webp
tags: [sticky]
canonical_url: 'https://learnbolts.com/completing-the-square/'
---

Hey there! Today we are going to solve the following equations using completing the square method.

Based on the steps used in learning completing the square method, we can solve quadratic equations with it.

Here are the questions we are going to solve:
1. $\color{blue}{6x^2\,+ 11x-35 = 0 }$
2. $\color{red}{x^2\, - 5x-14 = 0 }$
3. $\color{green}{2x^2\,+ -7x-15 = 0 }$

### Question 1

$\color{blue}{6x^2\,+ 11x-35 = 0 }$

#### STEP 1: Add $35$ to both sides of the equation

${6x^2\,+ 11x-35+35 = 0+35 }$

${6x^2\,+ 11x = 35 }$

#### Step 2: Divide both sides by the coefficient of ${x^2}$

$\frac{6x^2}{6}+\frac{11x}{6} = \frac{35}{6}$

$ x^2+\frac{11x}{6} = \frac{35}{6}$

#### Step 3: Multiply $\frac{1}{2}$ by $\frac{11}{6}$
$\frac{11}{6}\times \frac{1}{2} = \frac{11}{12}$ 

#### Step 4: Square the result and sum it to both sides
$x^2 + \frac{11x}{6} + (\frac{11}{12})^2 = \frac{35}{6} + (\frac{11}{12})^2$

$x^2 + \frac{11x}{6} + \frac{121}{144} = \frac{35}{6} + \frac{121}{144}$

#### Step 5: Factorize the LHS and find the LCM of the RHS
1. The LHS = $ (x \,+ \frac{11}{12})^2$

2. The RHS = $\frac{(35\,\times 24) + 121 }{144}$

$(x \,+ \frac{11}{12})^2= \frac{840 + 121 }{144}$

$(x \,+ \frac{11}{12})^2= \frac{961}{144}$

#### Step 6: Move the square on the LHS to the RHS
$ Example: a^2 = b$

$ a = \sqrt{b}$

Using the example above to solve the equation

$ x \,+ \frac{11}{12}= \sqrt{\frac{961}{144}}$

$x \,+ \frac{11}{12} = \frac{\sqrt{961}}{\sqrt{144}}$

#### Step 7: Find the square root of $ \sqrt{961}$ and ${\sqrt{144}}$
${\sqrt{961}} = 31$

$\sqrt{144} = 12$

#### Step 8: By simplification, the equation becomes....

$x \,+ \frac{11}{12} = \pm\frac{31}{12}$

$x = -\frac{11}{12} \pm\frac{31}{12}$

#### Step 9: Split $\pm$ into $+\, and\, -$

$$x = \frac{-11\; +{31}}{12}
\quad or \quad
x = \frac{-11\; -31 }{12}$$

$$x =  \frac{20}{12}
\quad or \quad x =  \frac{-41}{12}$$

#### Step 10: Reduce the fractions to the lowest term 

$$x = {\frac{5}{3}}
 \quad or \quad
  x = \frac{-41}{12}$$


#### The values of $x$ are:

$$\color{red}{x = \frac{5}{3},  \frac{-41}{12}}$$

### Question 2

$\color{blue}{x^2\,+ -5x-14 = 0 }$

#### STEP 1: Add $14$ to both sides of the equation

${x^2\,-5x-14+14 = 14 }$

${x^2\,-5x = 14 }$

#### Step 3: Multiply $\frac{1}{2}$ by $5$
$5\times \frac{1}{2} = \frac{5}{2}$ 

#### Step 4: Square the result and sum it to both sides
$x^2 - {5x} + (\frac{5}{2})^2 = 14 + (\frac{5}{2})^2$

$x^2 -5x + \frac{25}{4} = 14 + \frac{25}{4}$

#### Step 5: Factorize the LHS and find the LCM of the RHS
1. The LHS = $ (x \,- \frac{5}{2})^2$

2. The RHS = $\frac{(14\,\times 4) + 25 }{4}$

$(x \,- \frac{5}{2})^2= \frac{81}{4}$

#### Step 6: Move the square on the LHS to the RHS
$ Example: a^2 = b$

$ a = \sqrt{b}$

Using the example above to solve the equation

$ x \,- \frac{5}{2}= \sqrt{\frac{81}{4}}$

$x \,- \frac{5}{2} = \frac{\sqrt{81}}{\sqrt{4}}$

#### Step 7: Find the square root of $ \sqrt{81}$ and ${\sqrt{4}}$
${\sqrt{81}} = 9$

$\sqrt{4} = 2$

#### Step 8: By simplification, the equation becomes....

$x \,- \frac{5}{2} = \pm\frac{9}{2}$

$x = \frac{5}{2} \pm\frac{9}{2}$

#### Step 9: Split $\pm$ into $+\, and\, -$

$$x = \frac{5\; +{9}}{2}
\quad or \quad
x = \frac{5\; -9}{2}$$

$$x =  \frac{14}{2}
\quad or \quad x =  \frac{-4}{2}$$

#### Step 10: Reduce the fractions to the lowest term 

$$x = 7
 \quad or \quad
  x = -2$$


#### The values of $x$ are:

$$\color{blue}{x = 7,  -2}$$

### Question 3

$\color{green}{2x^2\,+ -7x-15 = 0 }$

#### STEP 1: Add $15$ to both sides of the equation

${2x^2\,-7x-15+15 = 0+15 }$

${2x^2\,-7x = 15 }$

#### Step 2: Divide both sides by the coefficient of ${x^2}$

$\frac{2x^2}{2}-\frac{7x}{2} = \frac{15}{2}$

$ x^2-\frac{7x}{2} = \frac{15}{2}$

#### Step 3: Multiply $\frac{1}{2}$ by $\frac{7}{2}$
$\frac{7}{2}\times \frac{1}{2} = \frac{7}{4}$ 

#### Step 4: Square the result and sum it to both sides
$x^2 - \frac{7x}{2} + (\frac{7}{4})^2 = \frac{15}{2} + (\frac{7}{4})^2$

$x^2 - \frac{7x}{2} + \frac{49}{16} = \frac{15}{2} + \frac{49}{16}$

#### Step 5: Factorize the LHS and find the LCM of the RHS
1. The LHS = $ (x \,- \frac{7}{4})^2$

2. The RHS = $\frac{(8\,\times 15) + 49 }{16}$

$(x \,- \frac{7}{4})^2= \frac{120 + 49 }{16}$

$(x \,- \frac{7}{4})^2= \frac{169}{16}$

#### Step 6: Move the square on the LHS to the RHS
$ Example: a^2 = b$

$ a = \sqrt{b}$

Using the example above to solve the equation

$ x \,- \frac{7}{4}= \sqrt{\frac{169}{16}}$

$x \,- \frac{7}{4} = \frac{\sqrt{961}}{\sqrt{16}}$

#### Step 7: Find the square root of $ \sqrt{169}$ and ${\sqrt{16}}$
${\sqrt{169}} = 13$

$\sqrt{16} = 12$

#### Step 8: By simplification, the equation becomes....

$x \,- \frac{7}{4} = \pm\frac{13}{4}$

$x = \frac{7}{4} \pm\frac{13}{4}$

#### Step 9: Split $\pm$ into $+\, and\, -$

$$x = \frac{7\; +{13}}{4}
\quad or \quad
x = \frac{7\; -13 }{4}$$

$$x =  \frac{20}{4}
\quad or \quad x =  \frac{-6}{4}$$

#### Step 10: Reduce the fractions to the lowest term 

$$x = 5
 \quad or \quad
  x = \frac{-3}{2}$$


#### The values of $x$ are:

$$\color{green}{x = 5,  \frac{-3}{2}}$$

To solve equations using quadratic formula method [click on the link](../quadratic-formula-example/)