---
layout: post
title:  "How to proof the quadratic formula | algebra | coolmath | polynomial | science"
author: sal
categories: [ maths ]
image: assets/images/Class-10-Quadratic-Equation-1.jpg
tags: [maths]
---

Hello! have you ever tried solving a quadratic equation using the quadratic formula, and wondered how the formula was proved. 

In this tutorial I'm going to teach you how you can prove the quadratic formula aka almighty formula.

The formula for a quadratic equation is:

$$\color{tan}{x} = \frac{-b\; \pm\sqrt{\color{Orchid}{b^2}\, -\color{red}{4ac}} }{\color{cyan}{2a}}$$

In proving the formula, we are going to use a sample equation

>$$ \color{red}{a}\color{tan}{x^2}\, + \color{Orchid}{b}\color{tan}{x}+\color{cyan}{c}  = \color{orange}{0}$$

Using <b>Completing the square method</b> to proving the formula
#### Step 1: Moving "$\color{cyan}{c}$" to the RHS of the equation

$ax^2\, +bx = -c$

##### Step 2: Divide both sides by the coefficient of $\color{tan}{x^2}$

$\frac{ax^2}{a}+\frac{bx}{a} = \frac{-c}{a}$

$ x^2+\frac{bx}{a} = \frac{-c}{a}$

##### Step 3: Multiply $\frac{1}{2}$ by $\frac{bx}{a}$
$\frac{bx}{a}\times \frac{1}{2} = \frac{bx}{2a}$ 

##### Step 4: Square the result and sum it to both sides
$x^2 + \frac{bx}{a} + (\frac{b}{2a})^2 = \frac{-c}{a} + (\frac{b}{2a})^2$

$x^2+\frac{bx}{a} + (\frac{b}{2a})^2 = \frac{-c}{a} + \frac{b^2}{4a^2}$

##### Step 5: Factorize the LHS and find the LCM of the RHS
1. The LHS = $ (x \,+ \frac{b}{2a})^2$

2. The RHS = $\frac{(-c\,\times 4a) + b^2 }{4a^2}$

 $ (x \,+ \frac{b}{2a})^2= \frac{(-4ac) + b^2 }{4a^2}$

##### Step 6: Move the square on the LHS to the RHS
$ Example: a^2 = b$

$ a = \sqrt{b}$

Using the example above to solve the equation

$ x \,+ \frac{b}{2a}= \sqrt{\frac{(-4ac) + b^2 }{4a^2}}$

$x \,+ \frac{b}{2a} = \frac{\sqrt{b^2 -4ac }}{\sqrt{4a^2}}$

##### Step 7: Find the square root of $ \sqrt{4a^2}$

$\sqrt{4a^2} = 2a$

##### Step 8: By simplification, the equation becomes....

$x \,+ \frac{b}{2a} = \pm\frac{\sqrt{b^2 -4ac }}{2a}$

$x = -\frac{b}{2a} \pm\frac{\sqrt{b^2 -4ac }}{2a}$

##### Step 9: Solve the equation by making $\color{cyan}{2a}$ the LCM

$$\color{tan}{x} = \frac{-b\; \pm\sqrt{\color{Orchid}{b^2}\, -\color{red}{4ac}} }{\color{cyan}{2a}}$$

<code>Hence the proof.</code>

#### For examples on how to use the formula, click on the link below

[Quadratic equations Examples](../quadratic-formula-example/)